Some more work on erase correctness.

LogRel/PseudoType.v
@@ -46,6 +46,57 @@ Fixpoint repEmulCtx (Γ : PEnv) : Env :=
     | pevar Γ τ => evar (repEmulCtx Γ) (repEmul τ)
   end.
 
+Lemma repEmulCtx_works {Γ i τ} :
+  ⟪ i : τ p∈ Γ ⟫ →
+  ⟪ i : repEmul τ ∈ repEmulCtx Γ ⟫.
+Proof.
+  induction 1; eauto using GetEvar. 
+Qed.
+
+Fixpoint embed (τ : Ty) : PTy :=
+  match τ with
+    | tarr τ₁ τ₂ => ptarr (embed τ₁) (embed τ₂)
+    | tunit => ptunit
+    | tbool => ptbool
+    | tprod τ₁ τ₂ => ptprod (embed τ₁) (embed τ₂)
+    | tsum τ₁ τ₂ => ptsum (embed τ₁) (embed τ₂)
+  end.
+
+Fixpoint embedCtx (Γ : Env) : PEnv :=
+  match Γ with
+      empty => pempty
+    | evar Γ τ => pevar (embedCtx Γ) (embed τ)
+  end.
+
+Lemma embedCtx_works {Γ i τ} :
+  ⟪ i : τ ∈ Γ ⟫ →
+  ⟪ i : embed τ p∈ embedCtx Γ ⟫.
+Proof.
+  induction 1; eauto using GetEvarP. 
+Qed.
+
+Lemma embedCtx_works_inv {Γ i τ} :
+  ⟪ i : τ p∈ embedCtx Γ ⟫ →
+  exists τ', τ = embed τ' ∧ ⟪ i : τ' ∈ Γ ⟫.
+Proof.
+  revert i τ. induction Γ; intros i τ' iτ; simpl in *; inversion iτ; subst.
+  - exists τ; intuition.
+  - destruct (IHΓ _ _ H3) as [τ'' [eq ty]].
+    exists τ''; intuition; eauto using GetEvarP. 
+Qed.
+
+Lemma repEmul_embed_leftinv τ :
+  repEmul (embed τ) = τ.
+Proof.
+  induction τ; simpl; try f_equal; intuition.
+Qed.
+
+Lemma repEmulCtx_embedCtx_leftinv Γ :
+  repEmulCtx (embedCtx Γ) = Γ.
+Proof.
+  induction Γ; simpl; try f_equal; eauto using repEmul_embed_leftinv.
+Qed.
+
 Lemma getevar_repEmulCtx {i τ Γ} :
   ⟪ i : τ ∈ repEmulCtx Γ ⟫ →
   exists τ', ⟪ i : τ' p∈ Γ ⟫ ∧ τ = repEmul τ'.
